Drop bucket array size condition from WFImp

Hashmap/DHashMap/AdditionalOperations.lean
@@ -26,18 +26,18 @@ open Internal.Raw
 
 theorem WF.filterMap [BEq α] [Hashable α] {m : Raw α β} (h : m.WF) {f : (a : α) → β a → Option (δ a)} :
     (m.filterMap f).WF := by
-  simpa only [filterMap_eq h] using .wf (Raw₀.filterMap f ⟨m, h.size_buckets_pos⟩).2 (Internal.Raw.WFImp.filterMap h.out)
+  simpa only [filterMap_eq h] using .wf (Raw₀.filterMap f ⟨m, h.size_buckets_pos⟩).2 (Raw₀.wfImp_filterMap (WF.out h))
 
 theorem WF.map [BEq α] [Hashable α] {m : Raw α β} (h : m.WF) {f : (a : α) → β a → δ a} :
     (m.map f).WF := by
-  simpa only [map_eq h] using .wf (Raw₀.map f ⟨m, h.size_buckets_pos⟩).2 (Internal.Raw.WFImp.map h.out)
+  simpa only [map_eq h] using .wf (Raw₀.map f ⟨m, h.size_buckets_pos⟩).2 (Raw₀.wfImp_map (WF.out h))
 
 end Raw
 
 @[inline] def filterMap [BEq α] [Hashable α] (f : (a : α) → β a → Option (δ a)) (m : DHashMap α β) : DHashMap α δ :=
-  ⟨Raw₀.filterMap f ⟨m.1, m.2.size_buckets_pos⟩, .wf (Raw₀.filterMap f ⟨m.1, m.2.size_buckets_pos⟩).2 (Internal.Raw.WFImp.filterMap m.2.out)⟩
+  ⟨Raw₀.filterMap f ⟨m.1, m.2.size_buckets_pos⟩, .wf (Raw₀.filterMap f ⟨m.1, m.2.size_buckets_pos⟩).2 (Raw₀.wfImp_filterMap (Raw.WF.out m.2))⟩
 
 @[inline] def map [BEq α] [Hashable α] (f : (a : α) → β a → δ a) (m : DHashMap α β) : DHashMap α δ :=
-  ⟨Raw₀.map f ⟨m.1, m.2.size_buckets_pos⟩, .wf (Raw₀.map f ⟨m.1, m.2.size_buckets_pos⟩).2 (Internal.Raw.WFImp.map m.2.out)⟩
+  ⟨Raw₀.map f ⟨m.1, m.2.size_buckets_pos⟩, .wf (Raw₀.map f ⟨m.1, m.2.size_buckets_pos⟩).2 (Raw₀.wfImp_map (Raw.WF.out m.2))⟩
 
 end Std.DHashMap
